theory/Static_Communication_Analysis.thy
@@ -4,7 +4,7 @@ begin
 
 fun proc_legacy_unsafe :: "control_path \<Rightarrow> control_path" where
   "proc_legacy_unsafe [] = []" |
-  "proc_legacy_unsafe (.l # \<pi>) = `l # []" |
+  "proc_legacy_unsafe (.l # \<pi>) = (*maybe just [] instead?  *) `l # []" |
   "proc_legacy_unsafe (`l # \<pi>) = `l # (proc_legacy_unsafe \<pi>)" |
   "proc_legacy_unsafe (\<upharpoonleft>\<bar>l # \<pi>) = \<upharpoonleft>\<bar>l # (proc_legacy_unsafe \<pi>)" |
   "proc_legacy_unsafe (\<upharpoonleft>:l # \<pi>) = \<upharpoonleft>:l # (proc_legacy_unsafe \<pi>)" |
@@ -57,10 +57,7 @@ inductive two_paths_exclusive :: "control_path \<Rightarrow> control_path \<Righ
       (proc_legacy \<pi>\<^sub>1) = Some \<pi>\<^sub>1l;
       (proc_legacy \<pi>\<^sub>2) = Some \<pi>\<^sub>2l;
 
-      (* better? *)
-      (proc_legacy \<pi>\<^sub>1l) = Some \<pi>\<^sub>1l';
-      (proc_legacy \<pi>\<^sub>2l) = Some \<pi>\<^sub>2l';
-      \<not> (two_paths_ordered \<pi>\<^sub>1l' \<pi>\<^sub>2l')
+      \<not> (two_paths_ordered \<pi>\<^sub>1l \<pi>\<^sub>2l)
     \<rbrakk> \<Longrightarrow>
     two_paths_exclusive \<pi>\<^sub>1 \<pi>\<^sub>2
   " |
@@ -73,6 +70,13 @@ inductive two_paths_exclusive :: "control_path \<Rightarrow> control_path \<Righ
       (proc_spawn \<pi>\<^sub>1) = Some \<pi>\<^sub>1w;
       (proc_spawn \<pi>\<^sub>2) = Some \<pi>\<^sub>2w;
       two_paths_exclusive \<pi>\<^sub>1w \<pi>\<^sub>2w
+
+(*
+      exclusive (
+  .x .z
+  .x .y
+)
+*)
     \<rbrakk> \<Longrightarrow>
     two_paths_exclusive \<pi>\<^sub>1 \<pi>\<^sub>2
   "
@@ -84,6 +88,7 @@ lemma two_paths_exclusive_preserved_under_pop: "
  apply (erule two_paths_exclusive.cases; auto)
   apply (simp add: two_paths_exclusive.Refl)
   apply (cases l; auto)
+   apply (simp add: two_paths_ordered_def)
   apply (cases l; auto)
 done
 
@@ -130,66 +135,14 @@ lemma two_paths_exclusive_commut: "
 done
 
 
-lemma two_paths_exclusive_and_unordered_implies_exclusive_or_prefix_under_backtrack': "
-       \<not> prefix \<pi>\<^sub>1 \<pi>\<^sub>2 \<Longrightarrow>
-       \<not> prefix \<pi>\<^sub>2 \<pi>\<^sub>1 \<Longrightarrow>
-       proc_legacy (\<pi>\<^sub>1 ;; l) = Some \<pi>\<^sub>2l \<Longrightarrow>
-       proc_legacy \<pi>\<^sub>2 = Some \<pi>\<^sub>2l \<Longrightarrow>
-       proc_spawn (\<pi>\<^sub>1 ;; l) = Some \<pi>\<^sub>1w \<Longrightarrow> proc_spawn \<pi>\<^sub>2 = Some \<pi>\<^sub>2w \<Longrightarrow> two_paths_exclusive \<pi>\<^sub>1w \<pi>\<^sub>2w \<Longrightarrow> two_paths_exclusive \<pi>\<^sub>1 \<pi>\<^sub>2
-"
-apply ((case_tac "\<pi>\<^sub>2" rule: proc_legacy.cases); auto)
-apply ((case_tac "\<pi>\<^sub>1 ;; l" rule: proc_legacy.cases); auto)
-apply (rename_tac x)
-apply (case_tac "\<pi>\<^sub>1" rule: proc_legacy.cases)
-defer
-apply auto[1]
-apply auto[1]
-apply auto[1]
-apply auto[1]
-apply auto[1]
-apply auto[1]
-apply auto[1]
-apply (case_tac "two_paths_exclusive \<pi> \<pi>\<^sub>2w"; auto?)
-
-(*
-.x y z g
-.x a b
-*)
-
-sorry
-
-(*
 lemma two_paths_exclusive_and_unordered_implies_exclusive_or_prefix_under_backtrack: "
   two_paths_exclusive (\<pi>\<^sub>1 ;; l) \<pi>\<^sub>2 \<Longrightarrow>
   \<not> prefix \<pi>\<^sub>1 \<pi>\<^sub>2 \<Longrightarrow>  \<not> prefix \<pi>\<^sub>2 \<pi>\<^sub>1 \<Longrightarrow>
   two_paths_exclusive \<pi>\<^sub>1 \<pi>\<^sub>2
 "
-(* 
-counter example:
-
-exclusive (  according to defs but shouldn't be
-  .x `y `a, 
-  .x .y `b 
-)
-
-not prefix (
-  x `y, 
-  x .y
-)
-
-not exclusive (.x `y, .x .y `b)
-
-original .x `y `a
-legacy   `x
-
-original .x .y `b
-legacy   `x
-
-*)
  apply (erule two_paths_exclusive.cases; auto)
  apply ((case_tac \<pi>\<^sub>1; auto; case_tac a; auto), (simp add: Base))
-using two_paths_exclusive_and_unordered_implies_exclusive_or_prefix_under_backtrack' by blast
-*)
+sorry
 
 lemma not_exclusive_with_process_split': "
   \<forall> x . two_paths_exclusive (\<pi> ;; .x) (\<pi> ;; `x) \<longrightarrow> False
